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Convergence

Theorem. Suppose xn → x and yn → y. Then xn + yn → x+ y.

Proof. Let ε > 0.

∃Nx : n > Na =⇒ |xn − x| < ε
2

xn → x1○
∃Ny : n > Ny =⇒ |yn − y| < ε

2
yn → y2○

Thus, for all n > N = max(Nx, Ny), we have

|xn + yn − (x+ y)| ≤ |xn − x|+ |yn − y| Triangle inequality

< ε 1○, 2○

Theorem. Suppose xn → x and yn → y. Then xnyn → xy.

Proof. First, let’s establish an identity:

xnyn − xy = xnyn − xny + xny − xy
= xn(yn − y) + y(xn − x)

= (xn − x+ x)(yn − y) + y(xn − x)

= (xn − x)(yn − y) + x(yn − y) + y(xn − x)

Now, let ε > 0.

∃Nx : n > Nx =⇒ |xn − x| <
√
ε

3
+

ε

3 |y|
xn → x1○

∃Ny : n > Ny =⇒ |yn − y| <
√
ε

3
+

ε

3 |x|
yn → y2○

Thus, for all n > N = max(Nx, Ny), we have

|xnyn − xy| = |(xn − x)(yn − y) + x(yn − y) + y(xn − x)| Identity above

≤ |xn − x| |yn − y|+ |x| |yn − y|+ |y| |xn − x| Triangle inequality

< ε
3

+ ε
3

+ ε
3

1○, 2○
= ε

In the construction of N above, note that we are assuming x, y 6= 0. If either is zero, the
second term in the sum can simply be omitted, as the corresponding term below is zero.

1



Theorem. Suppose xn → x, with xn 6= 0 for all n and x 6= 0. Then 1/xn → 1/x.

Proof. First, let us note that |a− b| < 1
2
|b| =⇒ |a| > 1

2
b. This is fairly obvious when you

think about it; to prove it, we can break the claim up into cases:

• b > 0 and a > b: a > b > b/2

• b > 0 and b > a: b− a < 1
2
b, so a > 1

2
b

The cases where b < 0 follow the same reasoning. Now, let ε > 0.

∃N1 : n > N1 =⇒ |xn − x| < 1
2
|x|2 ε xn → x1○

∃N2 : n > N2 =⇒ |xn − x| < 1
2
|x| xn → x2○

so that |xn| > 1
2
|x| 2○, see above3○

Thus, for all n > N = max(N1, N2), we have∣∣∣∣ 1

xn
− 1

x

∣∣∣∣ =

∣∣∣∣x− xnxnx

∣∣∣∣
≤ 2

|x|2
|xn − x| 3○

< ε 1○

Note that in this third theorem, the requirement that xn 6= 0 is unnecessary. As we see from
3○, if xn → x and x 6= 0, then there is an N such that xn 6= 0 for all n > N .

Continuity

The first two theorems are essentially the same as their sequence counterparts, but the
differences are worth paying attention to.

Theorem. Let the functions f and g be continuous at x0. Then h = f + g is continuous at
x0.

Proof. Let ε > 0.

∃δf : |x− x0| < δf =⇒ |f(x)− f(x0)| < ε
2

f continuous at x01○
∃δg : |x− x0| < δg =⇒ |g(x)− g(x0)| < ε

2
g continuous at x02○

Thus, for all x : |x− x0| < δ = min(δf , δg), we have

|h(x)− h(x0)| = |f(x) + g(x)− f(x0)− g(x0)| Def h

≤ |f(x)− f(x0)|+ |g(x)− g(x0)| Triangle inequality

≤ ε 1○, 2○

Theorem. Let the functions f and g be continuous at x0. Then h = f · g is continuous at
x0.
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Proof. Let ε > 0.

∃δf : |x− x0| < δf =⇒ |f(x)− f(x0)| <
√
ε

3
+

ε

3 |g(x0)|
f continuous at x01○

∃δg : |x− x0| < δg =⇒ |g(x)− g(x0)| <
√
ε

3
+

ε

3 |f(x0)|
g continuous at x02○

Thus, for all x : |x− x0| < δ = min(δf , δg), we have

|h(x)− h(x0)| = |f(x)g(x)− f(x0)g(x0)| Def h

≤ |{f(x)− f(x0)}{g(x)− g(x0)}|
+ |f(x0){g(x)− g(x0)}|
+ |g(x0){f(x)− f(x0)}| See earlier proof

< ε
3

+ ε
3

+ ε
3

1○, 2○
= ε

Theorem. Let the function f be continuous at x0 and the function g be continuous at f(x0).
Then h(x) = g(f(x)) is continuous at x0.

Proof. Let ε > 0.

∃η : |y − f(x0)| < η =⇒ |g(y)− g(f(x0))| < ε g continuous at f(x0)1○
∃δ : |x− x0| < δ =⇒ |f(x)− f(x0)| < η f continuous at x02○

Thus, for all x : |x− x0| < δ, we have

|h(x)− h(x0)| = |g(f(x))− g(f(x0))| Def h

< ε 2○ =⇒ 1○

Exercise: Write an R function n(eps) that returns the smallest N for which n > N =⇒
|f(xn)− f(x0)| < ε for xn = 21/n and f(x) = ex.

Conceptually, this is a three-part process:

1. Determine what xn is converging to. Here, xn → 1.
2. Determine the largest value of delta that satisfies e1+δ − e1 < ε.
3. Determine the smallest value of N such that 21/n − 1 < δ.

n <- function(eps) {

delta <- log(eps + exp(1)) - 1

ceiling(1/log2(1+delta))

}

n(0.01) ## 190

# Check solution

exp(2^(1/189)) - exp(1) ## 189 not good enough

exp(2^(1/190)) - exp(1) ## 190 within 0.01
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